theories/utils.v
@@ -1,0 +1,29 @@
+(** Useful general definitions **)
+(* (C) M. Bodin - see LICENSE.txt *)
+
+From mathcomp Require Import seq.
+
+Set Implicit Arguments.
+
+(** * An equivalent to [List.Forall], but in [Type] instead of [Prop]. **)
+
+Module TProp.
+
+Inductive Forall (A : Type) (P : A -> Type) : seq A -> Type :=
+  | Forall_nil : Forall P nil
+  | Forall_cons : forall e l, P e -> Forall P l -> Forall P (e :: l)
+  .
+
+Fixpoint max A l (F : Forall (fun (_ : A) => nat) l) : nat :=
+  match F with
+  | Forall_nil => 0
+  | Forall_cons _ _ n F => Nat.max n (max F)
+  end.
+
+Fixpoint map A P Q (f : forall a, P a -> Q a) (l : seq A) (F : Forall P l) : Forall Q l :=
+  match F with
+  | Forall_nil => Forall_nil _
+  | Forall_cons _ _ p F => Forall_cons _ (f _ p) (map _ f F)
+  end.
+
+End TProp.
